WIP: cached BoolExprNat -> AIG

LeanSAT/Heap.lean
@@ -12,6 +12,11 @@ theorem Array.push_get_old (as : Array α) (a : α) (h : i < as.size) : (as.push
 theorem Array.push_get_size (as : Array α) (a : α) : (as.push a)[as.size] = a := by
   simp [Array.push_get]
 
+theorem or_as_and (a b : Bool) : (!(!a && !b)) = (a || b) := by cases a <;> cases b <;> decide
+theorem xor_as_and (a b : Bool) : (!(a && b) && !(!a && !b)) = (xor a b) := by cases a <;> cases b <;> decide
+theorem beq_as_and (a b : Bool) : (!(a && !b) && !(!a && b)) = (a == b) := by cases a <;> cases b <;> decide
+theorem imp_as_and (a b : Bool) : (!(a && !b)) = (!a || b) := by cases a <;> cases b <;> decide
+
 /--
 A circuit node declaration. These are not recursive but instead contain indices into an `Env`.
 -/
@@ -25,9 +30,11 @@ inductive Decl where
   -/
   | atom (idx : Nat)
   /--
-  An AIG gate with configurable input nodes and polarity.
+  An AIG gate with configurable input nodes and polarity. `l` and `r` are the
+  input node indices while `linv` and `rinv` say whether there is an inverter on
+  the left or right input.
   -/
-  | gate (x y : Nat) (xpol ypol : Bool)
+  | gate (l r : Nat) (linv rinv : Bool)
   deriving BEq, Hashable, Repr
 
 /--
@@ -70,7 +77,7 @@ def Cache.insert (cache : Cache decls) (decl : Decl) : Cache (decls.push decl) :
   ⟨cache.val.insert decl decls.size, Cache.WF.push_cache cache.property⟩
 
 /--
-Lookup a `decl` in a `cache`. 
+Lookup a `decl` in a `cache`.
 
 If this returns `some i`, `Cache.find?_poperty` can be used to demonstrate: `decls[i] = decl`.
 -/
@@ -93,13 +100,13 @@ axiom Cache.find?_property {decls : Array Decl} {idx : Nat} (c : Cache decls) (d
 /--
 An `Array Decl` is a Direct Acyclic Graph (DAG) if this holds.
 -/
-def IsDag (decls : Array Decl) : Prop := ∀ i lhs rhs lpol rpol (h : i < decls.size), decls[i] = .gate lhs rhs lpol rpol → lhs < i ∧ rhs < i
+def IsDag (decls : Array Decl) : Prop := ∀ i lhs rhs linv rinv (h : i < decls.size), decls[i] = .gate lhs rhs linv rinv → lhs < i ∧ rhs < i
 
 /--
 The empty array is a DAG.
 -/
 theorem IsDag.empty : IsDag #[] := by
-  intro i lhs rhs lpol rpol h
+  intro i lhs rhs linv rinv h
   simp only [Array.size_toArray, List.length_nil] at h
   omega
 
@@ -153,11 +160,11 @@ where
     match h3 : decls[x] with
     | .const b => b
     | .atom v => assign.getD v false
-    | .gate lhs rhs lpol rpol =>
+    | .gate lhs rhs linv rinv =>
       have := h2 x _ _ _ _ h1 h3
       let lval := go lhs decls assign (by omega) h2
       let rval := go rhs decls assign (by omega) h2
-      xor lval lpol && xor rval rpol
+      xor lval linv && xor rval rinv
 
 /--
 Running `Env.denote.go` on a node that is within bounds of `decls` is equivalent to running it a bigger `decls` array.
@@ -179,54 +186,142 @@ theorem Env.denote.go_lt_push (x : Nat) (decls : Array Decl) (h1 : x < decls.siz
     . next heq2 => rw [h4, heq1] at heq2; injections
     . next heq2 => rw [h4, heq1] at heq2; injection heq2 with heq3; simp [heq3]
     . next heq2 => rw [h4, heq1] at heq2; injections
-  . next lhs1 rhs1 lpol1 rpol1 heq1 =>
+  . next lhs1 rhs1 linv1 rinv1 heq1 =>
     split
     . next heq2 => rw [h4, heq1] at heq2; injections
     . next heq2 => rw [h4, heq1] at heq2; injections
-    . next lhs2 rhs2 lpol2 rpol2 heq2 =>
+    . next lhs2 rhs2 linv2 rinv2 heq2 =>
       rw [heq1, heq2] at h4
-      injection h4 with lhseq rhseq lpoleq rpoleq
-      simp only [lhseq, lpoleq, rhseq, rpoleq]
-      have := inv x lhs1 rhs1 lpol1 rpol1 h1 heq1
+      injection h4 with lhseq rhseq linveq rinveq
+      simp only [lhseq, linveq, rhseq, rinveq]
+      have := inv x lhs1 rhs1 linv1 rinv1 h1 heq1
       apply ReflectSat.EvalAtAtoms.and_congr
       all_goals
         apply ReflectSat.EvalAtAtoms.xor_congr
         . apply denote.go_lt_push
           assumption
         . rfl
+termination_by sizeOf x
+
+theorem Env.denote.go_eq_of_env_eq (decls1 decls2 : Array Decl) {hdag1} {hdag2} {hbounds}
+    (hsize : decls1.size ≤ decls2.size)
+    (hidx : ∀ idx (h : idx < decls1.size), decls2[idx]'(by omega) = decls1[idx]'h) :
+    denote.go start decls2 assign (by omega) hdag2
+      =
+    denote.go start decls1 assign hbounds hdag1 := by
+  unfold denote.go
+  have hidx1 := hidx start hbounds
+  split
+  . next heq =>
+    rw [hidx1] at heq
+    split <;> simp_all
+  . next heq =>
+    rw [hidx1] at heq
+    split <;> simp_all
+  . next lhs rhs linv rinv heq =>
+    rw [hidx1] at heq
+    have foo := hdag1 start lhs rhs linv rinv hbounds heq
+    have hidx2 := hidx lhs (by omega)
+    have hidx3 := hidx rhs (by omega)
+    split
+    . simp_all
+    . simp_all
+    . simp_all
+      apply ReflectSat.EvalAtAtoms.and_congr
+      all_goals
+        apply ReflectSat.EvalAtAtoms.xor_congr
+        . apply Env.denote.go_eq_of_env_eq
+          . exact hidx
+          . exact hsize
+        . rfl
+termination_by sizeOf start
+
+theorem Env.denote.eq_of_env_eq (entry : Entrypoint) (newEnv : Env)
+    (hsize : entry.env.decls.size ≤ newEnv.decls.size)
+    (hidx : ∀ idx (h : idx < entry.env.decls.size), newEnv.decls[idx]'(by omega) = entry.env.decls[idx]'h)
+    {hbounds} :
+    denote ⟨newEnv, entry.start, hbounds⟩ assign
+      =
+    denote entry assign := by
+  unfold denote
+  apply Env.denote.go_eq_of_env_eq
+  exact hidx
+  exact hsize
+
+@[simp]
+theorem Env.denote_projected_entry {entry : Env.Entrypoint} :
+    denote ⟨entry.env, entry.start, entry.inv⟩ assign = denote entry assign := by
+  cases entry; simp
 
 /--
 Build an AIG gate in `env`. Note that his version is only meant for proving,
 for production purposes use `Env.mkGateCached` and equality theorems to this one.
 -/
-def Env.mkGate (lhs rhs : Nat) (lpol rpol : Bool) (env : Env) (hl : lhs < env.decls.size) 
+def Env.mkGate (lhs rhs : Nat) (linv rinv : Bool) (env : Env) (hl : lhs < env.decls.size)
     (hr : rhs < env.decls.size) : Env.Entrypoint :=
   let g := env.decls.size
-  let decls := env.decls.push (.gate lhs rhs lpol rpol)
+  let decls := env.decls.push (.gate lhs rhs linv rinv)
   let cache := env.cache.noUpdate
   have inv := by
-    intro i lhs rhs lpol rpol h1 h2
+    intro i lhs rhs linv rinv h1 h2
     simp only [decls, Array.push_get] at h2
     split at h2
     . apply env.inv <;> assumption
     . injections; omega
   ⟨{ env with decls, inv, cache }, g, by simp [g, decls]⟩
 
+
 /--
 `Env.mkGate` never shrinks the underlying AIG.
 -/
-theorem Env.mkGate_le_size (lhs rhs : Nat) (lpol rpol : Bool) (env : Env) hl hr
-    : env.decls.size ≤ (env.mkGate lhs rhs lpol rpol hl hr).env.decls.size := by
+theorem Env.mkGate_le_size (lhs rhs : Nat) (linv rinv : Bool) (env : Env) hl hr
+    : env.decls.size ≤ (env.mkGate lhs rhs linv rinv hl hr).env.decls.size := by
   simp_arith [mkGate]
+
+theorem Env.mkGate_decl_eq idx (h : idx < env.decls.size) {hbound} :
+    (mkGate lhs rhs linv rinv env hl hr).env.decls[idx]'hbound = env.decls[idx] := by
+  simp only [mkGate, Array.push_get]
+  split
+  . rfl
+  . contradiction
+
+@[simp]
+theorem Env.denote_mkGate :
+    denote (mkGate lhs rhs linv rinv env hl hr) assign
+      =
+    ((xor (denote ⟨env, lhs, hl⟩ assign) linv) && (xor (denote ⟨env, rhs, hr⟩ assign) rinv)) := by
+  conv =>
+    lhs
+    unfold denote denote.go
+  split
+  . next heq =>
+    rw [mkGate, Array.push_get_size] at heq
+    contradiction
+  . next heq =>
+    rw [mkGate, Array.push_get_size] at heq
+    contradiction
+  . next heq =>
+    rw [mkGate, Array.push_get_size] at heq
+    injection heq with heq1 heq2 heq3 heq4
+    simp
+    apply ReflectSat.EvalAtAtoms.and_congr
+    all_goals
+      apply ReflectSat.EvalAtAtoms.xor_congr
+      . unfold denote
+        simp only [heq1, heq2]
+        apply Env.denote.go_eq_of_env_eq
+        . intro idx h; apply mkGate_decl_eq
+        . apply mkGate_le_size
+      . simp only [heq3, heq4]
 
 /--
 Reusing an `Env.Entrypoint` to build an additional gate will never invalidate the entry node of
 the original entrypoint.
 -/
-theorem Env.lt_mkGate_size (e1 : Env.Entrypoint) (lhs rhs : Nat) (lpol rpol : Bool) hl hr
-    : e1.start < (e1.env.mkGate lhs rhs lpol rpol hl hr).env.decls.size := by
+theorem Env.lt_mkGate_size (e1 : Env.Entrypoint) (lhs rhs : Nat) (linv rinv : Bool) hl hr
+    : e1.start < (e1.env.mkGate lhs rhs linv rinv hl hr).env.decls.size := by
   have h1 := e1.inv
-  have h2 : e1.env.decls.size ≤ (e1.env.mkGate lhs rhs lpol rpol hl hr).env.decls.size :=
+  have h2 : e1.env.decls.size ≤ (e1.env.mkGate lhs rhs linv rinv hl hr).env.decls.size :=
     Env.mkGate_le_size _ _ _ _ _ _ _
   omega
 
@@ -234,9 +329,9 @@ theorem Env.lt_mkGate_size (e1 : Env.Entrypoint) (lhs rhs : Nat) (lpol rpol : Bo
 A version of `Env.mkGate` that uses the subterm cache in `Env`. This version is meant for
 programmming, for proving purposes use `Env.mkGate` and equality theorems to this one.
 -/
-def Env.mkGateCached (lhs rhs : Nat) (lpol rpol : Bool) (env : Env) (hl : lhs < env.decls.size)
+def Env.mkGateCached (lhs rhs : Nat) (linv rinv : Bool) (env : Env) (hl : lhs < env.decls.size)
     (hr : rhs < env.decls.size) : Env.Entrypoint :=
-  let decl := .gate lhs rhs lpol rpol
+  let decl := .gate lhs rhs linv rinv
   match h:env.cache.find? decl with
   | some gate =>
     ⟨env, gate, by apply Cache.find?_bounds _ _ h⟩
@@ -245,7 +340,7 @@ def Env.mkGateCached (lhs rhs : Nat) (lpol rpol : Bool) (env : Env) (hl : lhs < 
     let decls := env.decls.push decl
     let cache := Cache.insert env.cache decl
     have inv := by
-      intro lhs rhs lpol rpol i h1 h2
+      intro lhs rhs linv rinv i h1 h2
       simp only [decls] at *
       simp only [Array.push_get] at h2
       split at h2
@@ -254,15 +349,37 @@ def Env.mkGateCached (lhs rhs : Nat) (lpol rpol : Bool) (env : Env) (hl : lhs < 
     ⟨{ env with decls, inv, cache }, g, by simp [g, decls]⟩
 
 /--
+`Env.mkGateCached` never shrinks the underlying AIG.
+-/
+theorem Env.mkGateCached_le_size (lhs rhs : Nat) (linv rinv : Bool) (env : Env) hl hr
+    : env.decls.size ≤ (env.mkGateCached lhs rhs linv rinv hl hr).env.decls.size := by
+  dsimp [mkGateCached]
+  split
+  . simp
+  . simp_arith
+
+/--
+Reusing an `Env.Entrypoint` to build an additional gate will never invalidate the entry node of
+the original entrypoint.
+-/
+theorem Env.lt_mkGateCached_size (e1 : Env.Entrypoint) (lhs rhs : Nat) (linv rinv : Bool) hl hr
+    : e1.start < (e1.env.mkGateCached lhs rhs linv rinv hl hr).env.decls.size := by
+  have h1 := e1.inv
+  have h2 : e1.env.decls.size ≤ (e1.env.mkGateCached lhs rhs linv rinv hl hr).env.decls.size :=
+    Env.mkGateCached_le_size _ _ _ _ _ _ _
+  omega
+
+/--
 The central equality theorem between `mkGateCached` and `mkGate`.
 -/
-theorem Env.mkGateCached_eval_eq_mkGate_eval (lhs rhs : Nat) (lpol rpol : Bool) (env : Env) (hl : lhs < env.decls.size)
-    (hr : rhs < env.decls.size) : denote (env.mkGateCached lhs rhs lpol rpol hl hr) assign = denote (env.mkGate lhs rhs lpol rpol hl hr) assign := by
+theorem Env.mkGateCached_eval_eq_mkGate_eval (lhs rhs : Nat) (linv rinv : Bool) (env : Env) (hl : lhs < env.decls.size)
+    (hr : rhs < env.decls.size) :
+    denote (env.mkGateCached lhs rhs linv rinv hl hr) assign = denote (env.mkGate lhs rhs linv rinv hl hr) assign := by
   simp only [mkGate, mkGateCached]
   split
   . next heq1 =>
     unfold denote denote.go
-    have h1 := Cache.find?_property env.cache (.gate lhs rhs lpol rpol) heq1
+    have h1 := Cache.find?_property env.cache (.gate lhs rhs linv rinv) heq1
     simp only [Array.size_push, Nat.lt_succ_self]
     split
     . next heq2 => rw [h1] at heq2; injections
@@ -273,8 +390,8 @@ theorem Env.mkGateCached_eval_eq_mkGate_eval (lhs rhs : Nat) (lpol rpol : Bool) 
       . next heq3 => rw [Array.push_get_size] at heq3; injections
       . next heq3 =>
         rw [Array.push_get_size] at heq3;
-        injection heq3 with lhseq rhseq lpoleq rpoleq
-        simp only [lhseq, lpoleq, rhseq, rpoleq]
+        injection heq3 with lhseq rhseq linveq rinveq
+        simp only [lhseq, linveq, rhseq, rinveq]
         simp_all only [Decl.gate.injEq]
         apply ReflectSat.EvalAtAtoms.and_congr
         all_goals
@@ -293,7 +410,7 @@ def Env.mkAtom (n : Nat) (env : Env) : Env.Entrypoint :=
   let decls := env.decls.push (.atom n)
   let cache := env.cache.noUpdate
   have inv := by
-    intro i lhs rhs lpol rpol h1 h2
+    intro i lhs rhs linv rinv h1 h2
     simp only [decls] at *
     simp only [Array.push_get] at h2
     split at h2
@@ -307,6 +424,28 @@ def Env.mkAtom (n : Nat) (env : Env) : Env.Entrypoint :=
 theorem Env.mkAtom_le_size (env : Env) (var : Nat)
     : env.decls.size ≤ (env.mkAtom var).env.decls.size := by
   simp_arith [mkAtom]
+
+theorem Env.mkAtom_decl_eq idx (h : idx < env.decls.size) {hbound} :
+    (mkAtom var env ).env.decls[idx]'hbound = env.decls[idx] := by
+  simp only [mkAtom, Array.push_get]
+  split
+  . rfl
+  . contradiction
+
+@[simp]
+theorem Env.denote_mkAtom : denote (mkAtom var env) assign = assign.getD var false := by
+  unfold denote denote.go
+  split
+  . next heq =>
+    rw [mkAtom, Array.push_get_size] at heq
+    contradiction
+  . next heq =>
+    rw [mkAtom, Array.push_get_size] at heq
+    injection heq with heq
+    rw [heq]
+  . next heq =>
+    rw [mkAtom, Array.push_get_size] at heq
+    contradiction
 
 /--
 A version of `Env.mkAtom` that uses the subterm cache in `Env`. This version is meant for
@@ -322,13 +461,23 @@ def Env.mkAtomCached (n : Nat) (env : Env) : Env.Entrypoint :=
     let decls := env.decls.push decl
     let cache := env.cache.insert decl
     have inv := by
-      intro i lhs rhs lpol rpol h1 h2
+      intro i lhs rhs linv rinv h1 h2
       simp only [decls] at *
       simp only [Array.push_get] at h2
       split at h2
       . apply env.inv <;> assumption
       . contradiction
   ⟨{ decls, inv, cache }, g, by simp [g, decls]⟩
+
+/--
+`Env.mkAtomCached` never shrinks the underlying AIG.
+-/
+theorem Env.mkAtomCached_le_size (env : Env) (var : Nat)
+    : env.decls.size ≤ (env.mkAtomCached var).env.decls.size := by
+  dsimp [mkAtomCached]
+  split
+  . simp
+  . simp_arith
 
 /--
 The central equality theorem between `mkAtomCached` and `mkAtom`.
@@ -364,7 +513,7 @@ def Env.mkConst (val : Bool) (env : Env) : Env.Entrypoint :=
   let decls := env.decls.push (.const val)
   let cache := env.cache.noUpdate
   have inv := by
-    intro i lhs rhs lpol rpol h1 h2
+    intro i lhs rhs linv rinv h1 h2
     simp only [decls] at *
     simp only [Array.push_get] at h2
     split at h2
@@ -372,12 +521,42 @@ def Env.mkConst (val : Bool) (env : Env) : Env.Entrypoint :=
     . contradiction
   ⟨{ decls, inv, cache }, g, by simp [g, decls]⟩
 
+theorem Env.mkConst_decl_eq idx (h : idx < env.decls.size) {hbound} :
+    (mkConst val env).env.decls[idx]'hbound = env.decls[idx] := by
+  simp only [mkConst, Array.push_get]
+  split
+  . rfl
+  . contradiction
+
 /--
 `Env.mkConst` never shrinks the underlying AIG.
 -/
 theorem Env.mkConst_le_size (env : Env) (val : Bool)
     : env.decls.size ≤ (env.mkConst val).env.decls.size := by
   simp_arith [mkConst]
+
+@[simp]
+theorem Env.denote_mkConst : denote (mkConst val env) assign = val := by
+  unfold denote denote.go
+  split
+  . next heq =>
+    rw [mkConst, Array.push_get_size] at heq
+    injection heq with heq
+    rw [heq]
+  . next heq =>
+    rw [mkConst, Array.push_get_size] at heq
+    contradiction
+  . next heq =>
+    rw [mkConst, Array.push_get_size] at heq
+    contradiction
+
+@[simp]
+theorem Env.denote_mkConst_lt (entry : Env.Entrypoint) {h} :
+    denote ⟨(mkConst val entry.env).env, entry.start, h⟩ assign = denote entry assign :=  by
+  apply Env.denote.go_eq_of_env_eq
+  . intro idx h
+    apply mkConst_decl_eq
+  . apply mkConst_le_size
 
 /--
 Reusing an `Env.Entrypoint` to build an additional constant will never invalidate the entry node of
@@ -403,13 +582,33 @@ def Env.mkConstCached (val : Bool) (env : Env) : Env.Entrypoint :=
     let decls := env.decls.push decl
     let cache := env.cache.insert decl
     have inv := by
-      intro i lhs rhs lpol rpol h1 h2
+      intro i lhs rhs linv rinv h1 h2
       simp only [decls] at *
       simp only [Array.push_get] at h2
       split at h2
       . apply env.inv <;> assumption
       . contradiction
   ⟨{ decls, inv, cache }, g, by simp [g, decls]⟩
+
+/--
+`Env.mkConstCached` never shrinks the underlying AIG.
+-/
+theorem Env.mkConstCached_le_size (env : Env) (val : Bool)
+    : env.decls.size ≤ (env.mkConstCached val).env.decls.size := by
+  dsimp [mkConstCached]
+  split
+  . simp
+  . simp_arith
+
+/--
+Reusing an `Env.Entrypoint` to build an additional constant will never invalidate the entry node of
+the original entrypoint.
+-/
+theorem Env.lt_mkConstCached_size (e1 : Env.Entrypoint) : e1.start < (e1.env.mkConstCached val).env.decls.size := by
+  have h1 := e1.inv
+  have h2 : e1.env.decls.size ≤ (e1.env.mkConstCached val).env.decls.size :=
+    Env.mkConstCached_le_size _ _
+  omega
 
 /--
 The central equality theorem between `mkConstCached` and `mkConst`.
@@ -437,7 +636,6 @@ theorem Env.mkConstCached_eval_eq_mkConst_eval (val : Bool) (env : Env)
     . next heq2 => rw [h1] at heq2; injections
   . simp [denote]
 
--- TODO: implement cached version of this with cached functions and prove equivalent
 /--
 Turn a `BoolExprNat` into an AIG + entrypoint. Note that this version is only meant
 for proving purposes. For programming use `Env.ofBoolExprNatCached` and equality theorems.
@@ -445,7 +643,7 @@ for proving purposes. For programming use `Env.ofBoolExprNatCached` and equality
 def Env.ofBoolExprNat (expr : BoolExprNat) : Env.Entrypoint :=
   go expr Env.empty |>.val
 where
-  /-
+  /--
   This function contains a series of `have` statements that fulfill no obvious purpose.
   They are used to prove the `env.decls.size ≤ entry.env.decls.size` invariant of the return
   value with the final omega call in each case. This invariant is necessary as we recursively
@@ -465,11 +663,11 @@ where
        constEntry.env.mkGate
          constEntry.start
          exprEntry.start
-         true
          false
+         true
          constEntry.inv
          (by apply Env.lt_mkConst_size)
-      have := constEntry.env.mkGate_le_size _ _ true false constEntry.inv (by apply Env.lt_mkConst_size)
+      have := constEntry.env.mkGate_le_size _ _ false true constEntry.inv (by apply Env.lt_mkConst_size)
       ⟨ret, by dsimp [constEntry, ret] at *; omega⟩
     | .gate g lhs rhs =>
       let ⟨lhsEntry, _⟩ := go lhs env
@@ -483,34 +681,34 @@ where
           rhsEntry.env.mkGate
             lhsEntry.start
             rhsEntry.start
-            true
-            true
+            false
+            false
             h1
             rhsEntry.inv
-        have := rhsEntry.env.mkGate_le_size _ _ true true h1 rhsEntry.inv
+        have := rhsEntry.env.mkGate_le_size _ _ false false h1 rhsEntry.inv
         ⟨ret, by dsimp [ret] at *; omega⟩
       | .or =>
         -- x or y = true && (invert (invert x && invert y))
         let auxEntry :=
           rhsEntry.env.mkGate
             lhsEntry.start
-            rhsEntry.start 
-            false
-            false
+            rhsEntry.start
+            true
+            true
             h1
             rhsEntry.inv
-        have := rhsEntry.env.mkGate_le_size _ _ false false h1 rhsEntry.inv
+        have := rhsEntry.env.mkGate_le_size _ _ true true h1 rhsEntry.inv
         let constEntry := auxEntry.env.mkConst true
         have := auxEntry.env.mkConst_le_size true
         let ret :=
           constEntry.env.mkGate
             constEntry.start
             auxEntry.start
-            true
             false
+            true
             constEntry.inv
             (by apply Env.lt_mkConst_size)
-        have := constEntry.env.mkGate_le_size _ auxEntry.start true false constEntry.inv (by apply Env.lt_mkConst_size)
+        have := constEntry.env.mkGate_le_size _ auxEntry.start false true constEntry.inv (by apply Env.lt_mkConst_size)
         ⟨ret, by dsimp [auxEntry, constEntry, ret] at *; omega⟩
       | .xor =>
         -- x xor y = (invert (invert (x && y))) && (invert ((invert x) && (invert y)))
@@ -518,11 +716,11 @@ where
           rhsEntry.env.mkGate
             lhsEntry.start
             rhsEntry.start
-            true
-            true
+            false
+            false
             h1
             rhsEntry.inv
-        have := rhsEntry.env.mkGate_le_size _ _ true true h1 rhsEntry.inv
+        have := rhsEntry.env.mkGate_le_size _ _ false false h1 rhsEntry.inv
         have h3 : lhsEntry.start < aux1Entry.env.decls.size := by
           dsimp [aux1Entry] at *
           omega
@@ -530,20 +728,20 @@ where
           aux1Entry.env.mkGate
             lhsEntry.start
             rhsEntry.start
-            false
-            false
+            true
+            true
             h3
             (by apply Env.lt_mkGate_size)
-        have := aux1Entry.env.mkGate_le_size _ _ false false h3 (by apply Env.lt_mkGate_size)
+        have := aux1Entry.env.mkGate_le_size _ _ true true h3 (by apply Env.lt_mkGate_size)
         let ret :=
           aux2Entry.env.mkGate
             aux1Entry.start
             aux2Entry.start
-            false
-            false
+            true
+            true
             (by apply Env.lt_mkGate_size)
             aux2Entry.inv
-        have := aux2Entry.env.mkGate_le_size aux1Entry.start _ false false (by apply Env.lt_mkGate_size) aux2Entry.inv
+        have := aux2Entry.env.mkGate_le_size aux1Entry.start _ true true (by apply Env.lt_mkGate_size) aux2Entry.inv
         ⟨ret, by simp (config := { zetaDelta := true}) only at *; omega⟩
       | .beq =>
         -- a == b = (invert (a && (invert b))) && (invert ((invert a) && b))
@@ -551,11 +749,11 @@ where
           rhsEntry.env.mkGate
             lhsEntry.start
             rhsEntry.start
-            true
             false
+            true
             h1
             rhsEntry.inv
-        have := rhsEntry.env.mkGate_le_size _ _ true false h1 rhsEntry.inv
+        have := rhsEntry.env.mkGate_le_size _ _ false true h1 rhsEntry.inv
         have h3 : lhsEntry.start < aux1Entry.env.decls.size := by
           dsimp [aux1Entry] at *
           omega
@@ -563,44 +761,372 @@ where
           aux1Entry.env.mkGate
             lhsEntry.start
             rhsEntry.start
-            false
             true
+            false
             h3
             (by apply Env.lt_mkGate_size)
-        have := aux1Entry.env.mkGate_le_size _ _ false true h3 (by apply Env.lt_mkGate_size)
+        have := aux1Entry.env.mkGate_le_size _ _ true false h3 (by apply Env.lt_mkGate_size)
         let ret :=
           aux2Entry.env.mkGate
             aux1Entry.start
             aux2Entry.start
-            false
-            false
+            true
+            true
             (by apply Env.lt_mkGate_size)
             aux2Entry.inv
-        have := aux2Entry.env.mkGate_le_size aux1Entry.start _ false false (by apply Env.lt_mkGate_size) aux2Entry.inv
+        have := aux2Entry.env.mkGate_le_size aux1Entry.start _ true true (by apply Env.lt_mkGate_size) aux2Entry.inv
         ⟨ret, by simp (config := { zetaDelta := true}) only at *; omega⟩
       | .imp =>
         -- a -> b = true && (invert (a and (invert b)))
         let auxEntry :=
           rhsEntry.env.mkGate
             lhsEntry.start
-            rhsEntry.start 
-            true
+            rhsEntry.start
             false
+            true
             h1
             rhsEntry.inv
-        have := rhsEntry.env.mkGate_le_size _ _ true false h1 rhsEntry.inv
+        have := rhsEntry.env.mkGate_le_size _ _ false true h1 rhsEntry.inv
         let constEntry := mkConst true auxEntry.env
         have := auxEntry.env.mkConst_le_size true
         let ret :=
           constEntry.env.mkGate
             constEntry.start
             auxEntry.start
-            true
             false
+            true
             constEntry.inv
             (by apply Env.lt_mkConst_size)
-        have := constEntry.env.mkGate_le_size _ auxEntry.start true false constEntry.inv (by apply Env.lt_mkConst_size)
+        have := constEntry.env.mkGate_le_size _ auxEntry.start false true constEntry.inv (by apply Env.lt_mkConst_size)
         ⟨ret, by dsimp [auxEntry, constEntry, ret] at *; omega⟩
 
 
 #eval Env.ofBoolExprNat (.gate .and (.gate .and (.literal 0) (.literal 0)) (.gate .and (.literal 0) (.literal 0))) |>.env.decls
+
+theorem Env.ofBoolExprNat.go_decls_size_le (expr : BoolExprNat) (env : Env) :
+    env.decls.size ≤ (ofBoolExprNat.go expr env).val.env.decls.size := by
+  exact (ofBoolExprNat.go expr env).property
+
+theorem Env.ofBoolExprNat.go_decl_eq (idx) (env) (h : idx < env.decls.size) (hbounds) :
+    (ofBoolExprNat.go expr env).val.env.decls[idx]'hbounds = env.decls[idx] := by
+  induction expr generalizing env with
+  | const =>
+    simp only [go]
+    apply Env.mkConst_decl_eq
+  | literal =>
+    simp only [go]
+    apply Env.mkAtom_decl_eq
+  | not expr ih =>
+    simp only [go]
+    have := go_decls_size_le expr env
+    specialize ih env (by omega) (by omega)
+    -- TODO: I think I want a more general theorem here
+    simp [mkConst, mkAtom, mkGate, Array.push_get]
+    split
+    . split
+      . assumption
+      . omega
+    . omega
+  | gate g lhs rhs lih rih =>
+    have := go_decls_size_le lhs env
+    have := go_decls_size_le rhs (go lhs env).val.env
+    specialize lih env (by omega) (by omega)
+    specialize rih (go lhs env).val.env (by omega) (by omega)
+    cases g with
+    | and =>
+      -- TODO: other use case for simp lemma
+      simp only [go]
+      simp [mkGate, mkAtom, Array.push_get]
+      split
+      . simp [rih, lih]
+      . omega
+    | or =>
+      -- TODO: other use case for simp lemma
+      simp only [go]
+      simp [mkGate, mkAtom, mkConst, Array.push_get]
+      split
+      . split
+        . split
+          . simp [lih, rih]
+          . omega
+        . omega
+      . omega
+    | xor =>
+      -- TODO: other use case for simp lemma
+      simp only [go]
+      simp [mkGate, mkAtom, Array.push_get]
+      split
+      . split
+        . split
+          . simp [lih, rih]
+          . omega
+        . omega
+      . omega
+    | beq =>
+      -- TODO: other use case for simp lemma
+      simp only [go]
+      simp [mkGate, mkAtom, Array.push_get]
+      split
+      . split
+        . split
+          . simp [lih, rih]
+          . omega
+        . omega
+      . omega
+    | imp =>
+      -- TODO: other use case for simp lemma
+      simp only [go]
+      simp [mkGate, mkAtom, mkConst, Array.push_get]
+      split
+      . split
+        . split
+          . simp [lih, rih]
+          . omega
+        . omega
+      . omega
+
+@[simp]
+theorem Env.foo (entry : Entrypoint) {h}:
+    denote ⟨(ofBoolExprNat.go expr entry.env).val.env, entry.start, h⟩ assign
+      =
+    denote entry assign := by
+  apply Env.denote.eq_of_env_eq
+  . intro idx h
+    apply Env.ofBoolExprNat.go_decl_eq
+  . apply Env.ofBoolExprNat.go_decls_size_le
+
+/-
+denote
+  {
+    env :=
+      (mkGate (ofBoolExprNat.go lhs env).val.start (ofBoolExprNat.go rhs (ofBoolExprNat.go lhs env).val.env).val.start
+          false false (ofBoolExprNat.go rhs (ofBoolExprNat.go lhs env).val.env).val.env ⋯ ⋯).env,
+    start := (ofBoolExprNat.go lhs env).val.start,
+    inv := ⋯
+  }
+-/
+
+-- TODO: much of this requires theorems about ofBoolExprNat.go in the spirit of Env.denote_mkConst_lt
+theorem Env.ofBoolExprNatgo_eval_eq_eval (expr : BoolExprNat) (env : Env) (assign : List Bool) :
+    denote (Env.ofBoolExprNat.go expr env) assign = expr.eval assign := by
+  induction expr generalizing env with
+  | const => simp [ofBoolExprNat.go]
+  | literal => simp [ofBoolExprNat.go]
+  | not expr ih =>
+    simp [ofBoolExprNat.go]
+    rw [← ih]
+  | gate g lhs rhs lih rih =>
+    cases g with
+    | and =>
+      simp [ofBoolExprNat.go, Gate.eval, lih, rih]
+    | or =>
+      simp [ofBoolExprNat.go, Gate.eval]
+      rw [← or_as_and]
+      simp [lih, rih]
+    | xor =>
+      simp [ofBoolExprNat.go, Gate.eval]
+      rw [← xor_as_and]
+      apply ReflectSat.EvalAtAtoms.and_congr
+      . apply ReflectSat.EvalAtAtoms.not_congr
+        sorry
+      . apply ReflectSat.EvalAtAtoms.not_congr
+        apply ReflectSat.EvalAtAtoms.and_congr
+        . apply ReflectSat.EvalAtAtoms.not_congr
+          sorry
+        . apply ReflectSat.EvalAtAtoms.not_congr
+          sorry
+    | beq =>
+      simp [ofBoolExprNat.go, Gate.eval]
+      rw [← beq_as_and]
+      apply ReflectSat.EvalAtAtoms.and_congr
+      . apply ReflectSat.EvalAtAtoms.not_congr
+        sorry
+      . apply ReflectSat.EvalAtAtoms.not_congr
+        apply ReflectSat.EvalAtAtoms.and_congr
+        . apply ReflectSat.EvalAtAtoms.not_congr
+          sorry
+        . sorry
+    | imp =>
+      simp [ofBoolExprNat.go, Gate.eval]
+      rw [← imp_as_and]
+      simp [lih, rih]
+
+theorem Env.ofBoolExprNat_eval_eq_eval (expr : BoolExprNat) (assign : List Bool) :
+    denote (Env.ofBoolExprNat expr) assign = expr.eval assign := by
+  apply Env.ofBoolExprNatgo_eval_eq_eval
+
+-- lines such as: ⟨ret, by dsimp [auxEntry, constEntry, ret] at *; omega⟩
+-- are slow because of the high defeq degree
+-- TODO: ask leo how to fix this stuff
+set_option pp.oneline true in
+set_option trace.profiler true in
+/--
+Turn a `BoolExprNat` into an AIG + entrypoint. Note that this version is meant for programming
+purposes. For proving use `Env.ofBoolExprNat` and equality theorems.
+-/
+def Env.ofBoolExprNatCached (expr : BoolExprNat) : Env.Entrypoint :=
+  go expr Env.empty |>.val
+where
+  @[inherit_doc Env.ofBoolExprNat.go]
+  go (expr : BoolExprNat) (env : Env) : { entry : Env.Entrypoint // env.decls.size ≤ entry.env.decls.size } :=
+    match expr with
+    | .literal var => ⟨env.mkAtomCached var, (by apply Env.mkAtomCached_le_size)⟩
+    | .const val => ⟨env.mkConstCached val, (by apply Env.mkConstCached_le_size)⟩
+    | .not expr =>
+      -- ¬x = true && invert x
+      let ⟨exprEntry, _⟩ := go expr env
+      let constEntry := exprEntry.env.mkConstCached true
+      have := exprEntry.env.mkConstCached_le_size true
+      let ret :=
+       constEntry.env.mkGateCached
+         constEntry.start
+         exprEntry.start
+         false
+         true
+         constEntry.inv
+         (by apply Env.lt_mkConstCached_size)
+      have := constEntry.env.mkGateCached_le_size _ _ false true constEntry.inv (by apply Env.lt_mkConstCached_size)
+      ⟨ret, by dsimp [constEntry, ret] at *; omega⟩
+    | .gate g lhs rhs =>
+      let ⟨lhsEntry, _⟩ := go lhs env
+      let ⟨rhsEntry, _⟩ := go rhs lhsEntry.env
+      have h1 : lhsEntry.start < Array.size rhsEntry.env.decls := by
+        have := lhsEntry.inv
+        omega
+      match g with
+      | .and =>
+        let ret :=
+          rhsEntry.env.mkGateCached
+            lhsEntry.start
+            rhsEntry.start
+            false
+            false
+            h1
+            rhsEntry.inv
+        have := rhsEntry.env.mkGateCached_le_size _ _ false false h1 rhsEntry.inv
+        ⟨ret, by dsimp [ret] at *; omega⟩
+      | .or =>
+        -- x or y = true && (invert (invert x && invert y))
+        let auxEntry :=
+          rhsEntry.env.mkGateCached
+            lhsEntry.start
+            rhsEntry.start
+            true
+            true
+            h1
+            rhsEntry.inv
+        have := rhsEntry.env.mkGateCached_le_size _ _ true true h1 rhsEntry.inv
+        let constEntry := auxEntry.env.mkConstCached true
+        have := auxEntry.env.mkConstCached_le_size true
+        let ret :=
+          constEntry.env.mkGateCached
+            constEntry.start
+            auxEntry.start
+            false
+            true
+            constEntry.inv
+            (by apply Env.lt_mkConstCached_size)
+        have := constEntry.env.mkGateCached_le_size _ auxEntry.start false true constEntry.inv (by apply Env.lt_mkConstCached_size)
+        ⟨ret, by dsimp [auxEntry, constEntry, ret] at *; omega⟩
+      | .xor =>
+        -- x xor y = (invert (invert (x && y))) && (invert ((invert x) && (invert y)))
+        let aux1Entry :=
+          rhsEntry.env.mkGateCached
+            lhsEntry.start
+            rhsEntry.start
+            false
+            false
+            h1
+            rhsEntry.inv
+        have := rhsEntry.env.mkGateCached_le_size _ _ false false h1 rhsEntry.inv
+        have h3 : lhsEntry.start < aux1Entry.env.decls.size := by
+          dsimp [aux1Entry] at *
+          omega
+        let aux2Entry :=
+          aux1Entry.env.mkGateCached
+            lhsEntry.start
+            rhsEntry.start
+            true
+            true
+            h3
+            (by apply Env.lt_mkGateCached_size)
+        have := aux1Entry.env.mkGateCached_le_size _ _ true true h3 (by apply Env.lt_mkGateCached_size)
+        let ret :=
+          aux2Entry.env.mkGateCached
+            aux1Entry.start
+            aux2Entry.start
+            true
+            true
+            (by apply Env.lt_mkGateCached_size)
+            aux2Entry.inv
+        have := aux2Entry.env.mkGateCached_le_size aux1Entry.start _ true true (by apply Env.lt_mkGateCached_size) aux2Entry.inv
+        ⟨ret, by simp (config := { zetaDelta := true}) only at *; omega⟩
+      | .beq =>
+        -- a == b = (invert (a && (invert b))) && (invert ((invert a) && b))
+        let aux1Entry :=
+          rhsEntry.env.mkGateCached
+            lhsEntry.start
+            rhsEntry.start
+            false
+            true
+            h1
+            rhsEntry.inv
+        have := rhsEntry.env.mkGateCached_le_size _ _ false true h1 rhsEntry.inv
+        have h3 : lhsEntry.start < aux1Entry.env.decls.size := by
+          dsimp [aux1Entry] at *
+          omega
+        let aux2Entry :=
+          aux1Entry.env.mkGateCached
+            lhsEntry.start
+            rhsEntry.start
+            true
+            false
+            h3
+            (by apply Env.lt_mkGateCached_size)
+        have := aux1Entry.env.mkGateCached_le_size _ _ true false h3 (by apply Env.lt_mkGateCached_size)
+        let ret :=
+          aux2Entry.env.mkGateCached
+            aux1Entry.start
+            aux2Entry.start
+            true
+            true
+            (by apply Env.lt_mkGateCached_size)
+            aux2Entry.inv
+        have := aux2Entry.env.mkGateCached_le_size aux1Entry.start _ true true (by apply Env.lt_mkGateCached_size) aux2Entry.inv
+        ⟨ret, by simp (config := { zetaDelta := true}) only at *; omega⟩
+      | .imp =>
+        -- a -> b = true && (invert (a and (invert b)))
+        let auxEntry :=
+          rhsEntry.env.mkGateCached
+            lhsEntry.start
+            rhsEntry.start
+            false
+            true
+            h1
+            rhsEntry.inv
+        have := rhsEntry.env.mkGateCached_le_size _ _ false true h1 rhsEntry.inv
+        let constEntry := mkConstCached true auxEntry.env
+        have := auxEntry.env.mkConstCached_le_size true
+        let ret :=
+          constEntry.env.mkGateCached
+            constEntry.start
+            auxEntry.start
+            false
+            true
+            constEntry.inv
+            (by apply Env.lt_mkConstCached_size)
+        have := constEntry.env.mkGateCached_le_size _ auxEntry.start false true constEntry.inv (by apply Env.lt_mkConstCached_size)
+        ⟨ret, by dsimp [auxEntry, constEntry, ret] at *; omega⟩
+
+#eval Env.ofBoolExprNatCached (.gate .and (.gate .and (.literal 0) (.literal 0)) (.gate .and (.literal 0) (.literal 0))) |>.env.decls
+
+theorem Env.ofBoolExprCachedgo_eval_eq_ofBoolExprgo_eval (expr : BoolExprNat) (assign : List Bool) (env : Env) :
+    Env.denote (Env.ofBoolExprNatCached.go expr env).val assign = Env.denote (Env.ofBoolExprNat.go expr env).val assign := by
+  sorry
+
+theorem Env.ofBoolExprCached_eval_eq_ofBoolExpr_eval (expr : BoolExprNat) (assign : List Bool) :
+    Env.denote (Env.ofBoolExprNatCached expr) assign = Env.denote (Env.ofBoolExprNat expr) assign := by
+  unfold Env.ofBoolExprNatCached
+  rw [Env.ofBoolExprCachedgo_eval_eq_ofBoolExprgo_eval]
+  unfold Env.ofBoolExprNat
+  rfl
